more

Weidenbach_Book/IsaSAT/Relational_Pairing_Heaps.thy
@@ -307,7 +307,8 @@ proof -
     scores x = map_option score (hp_node_children x (a @ [Hp m w\<^sub>m ch\<^sub>m, Hp n w\<^sub>n ch\<^sub>n] @ b)))\<close> and
     dist2: \<open>distinct_mset (\<Sum>\<^sub># (mset_nodes `# xs + mset_nodes `# mset (a @ [Hp m w\<^sub>m ch\<^sub>m, Hp n w\<^sub>n ch\<^sub>n] @ b)))\<close> and
     others_empty: \<open>empty_outside (\<Sum>\<^sub># (mset_nodes `# xs + mset_nodes `# mset (a @ [Hp m w\<^sub>m ch\<^sub>m, Hp n w\<^sub>n ch\<^sub>n] @ b))) prevs\<close>
-       \<open>empty_outside (\<Sum>\<^sub># (mset_nodes `# xs + mset_nodes `# mset (a @ [Hp m w\<^sub>m ch\<^sub>m, Hp n w\<^sub>n ch\<^sub>n] @ b))) parents\<close>
+    \<open>empty_outside (\<Sum>\<^sub># (mset_nodes `# xs + mset_nodes `# mset (a @ [Hp m w\<^sub>m ch\<^sub>m, Hp n w\<^sub>n ch\<^sub>n] @ b))) parents\<close> and
+    incl: \<open>set_mset (\<Sum>\<^sub># (mset_nodes `# xs + mset_nodes `# mset (a @ [Hp m w\<^sub>m ch\<^sub>m, Hp n w\<^sub>n ch\<^sub>n] @ b))) \<subseteq> set_mset \<V>\<close>
     using assms unfolding encoded_hp_prop_list_def by auto
   have [simp]: \<open>distinct_mset (sum_list (map mset_nodes ch\<^sub>n) + sum_list (map mset_nodes ch\<^sub>m))\<close>
     \<open>distinct_mset (sum_list (map mset_nodes ch\<^sub>n) + sum_list (map mset_nodes b))\<close>
@@ -389,6 +390,7 @@ proof -
     apply (intro conjI impI allI)
     subgoal using assms unfolding encoded_hp_prop_list_def
       by (auto simp: ac_simps simp del: NOTIN_def[symmetric])
+    subgoal using incl by auto
     subgoal using nxts1
       by auto
     subgoal using prevs1
@@ -451,8 +453,8 @@ lemma encoded_hp_prop_list_link2:
   defines \<open>nxts' \<equiv> nxts\<^sub>0 (n := map_option node (option_hd b), m := map_option node (option_hd ch\<^sub>n))\<close>
   defines \<open>children' \<equiv> children (n := Some m)\<close>
   defines \<open>parents' \<equiv> (if ch\<^sub>n = [] then parents else parents(node (hd ch\<^sub>n) := None))(m := Some n)\<close>
-  assumes \<open>encoded_hp_prop_list (xs) (a @ [Hp m w\<^sub>m ch\<^sub>m, Hp n w\<^sub>n ch\<^sub>n] @ b) (prevs, nxts, children, parents, scores)\<close>
-  shows \<open>encoded_hp_prop_list xs (a @ [Hp n w\<^sub>n (Hp m w\<^sub>m ch\<^sub>m # ch\<^sub>n)] @ b)
+  assumes \<open>encoded_hp_prop_list \<V> (xs) (a @ [Hp m w\<^sub>m ch\<^sub>m, Hp n w\<^sub>n ch\<^sub>n] @ b) (prevs, nxts, children, parents, scores)\<close>
+  shows \<open>encoded_hp_prop_list \<V> xs (a @ [Hp n w\<^sub>n (Hp m w\<^sub>m ch\<^sub>m # ch\<^sub>n)] @ b)
        (prevs', nxts', children', parents', scores)\<close>
 proof -
   have dist: \<open>distinct_mset (sum_list (map mset_nodes ch\<^sub>m) + (sum_list (map mset_nodes ch\<^sub>n) +
@@ -484,7 +486,8 @@ proof -
     scores1: \<open>(\<forall>m\<in>#xs. \<forall>x\<in>#mset_nodes m. scores x = map_option score (hp_node x m))\<close> and
     dist2: \<open>distinct_mset (\<Sum>\<^sub># (mset_nodes `# xs + mset_nodes `# mset (a @ [Hp m w\<^sub>m ch\<^sub>m, Hp n w\<^sub>n ch\<^sub>n] @ b)))\<close> and
     others_empty: \<open>empty_outside (\<Sum>\<^sub># (mset_nodes `# xs + mset_nodes `# mset (a @ [Hp m w\<^sub>m ch\<^sub>m, Hp n w\<^sub>n ch\<^sub>n] @ b))) prevs\<close>
-      \<open>empty_outside (\<Sum>\<^sub># (mset_nodes `# xs + mset_nodes `# mset (a @ [Hp m w\<^sub>m ch\<^sub>m, Hp n w\<^sub>n ch\<^sub>n] @ b))) parents\<close>
+      \<open>empty_outside (\<Sum>\<^sub># (mset_nodes `# xs + mset_nodes `# mset (a @ [Hp m w\<^sub>m ch\<^sub>m, Hp n w\<^sub>n ch\<^sub>n] @ b))) parents\<close> and
+    incl: \<open>set_mset (\<Sum>\<^sub># (mset_nodes `# xs + mset_nodes `# mset (a @ [Hp m w\<^sub>m ch\<^sub>m, Hp n w\<^sub>n ch\<^sub>n] @ b))) \<subseteq> set_mset \<V>\<close>
     using assms unfolding encoded_hp_prop_list_def prod.simps by clarsimp_all
   have [simp]: \<open>distinct_mset (sum_list (map mset_nodes ch\<^sub>n) + sum_list (map mset_nodes ch\<^sub>m))\<close>
     \<open>distinct_mset (sum_list (map mset_nodes ch\<^sub>n) + sum_list (map mset_nodes b))\<close>
@@ -589,6 +592,7 @@ proof -
     apply (intro conjI impI allI)
     subgoal using assms unfolding encoded_hp_prop_list_def
       by (auto simp: ac_simps simp del: NOTIN_def[symmetric])
+    subgoal using incl by auto
     subgoal using nxts1
       apply (cases a rule: rev_cases)
       apply auto
@@ -649,25 +653,38 @@ qed
 
 (*TODO this seems to be never used in the refinement part*)
 definition encoded_hp_prop_list_conc
-  :: "'a::linorder set \<times> ('a, 'b) hp_fun \<times> 'a option \<Rightarrow>
+  :: "'a::linorder multiset \<times> ('a, 'b) hp_fun \<times> 'a option \<Rightarrow>
      'a multiset \<times> ('a, 'b) hp option \<Rightarrow> bool"
   where
-  \<open>encoded_hp_prop_list_conc = (\<lambda>(\<V>, arr, h) (\<V>', x). \<V> = set_mset \<V>' \<and>
-  (case x of None \<Rightarrow> encoded_hp_prop_list {#} ([]:: ('a, 'b) hp list) arr \<and> h = None
-  | Some x \<Rightarrow> encoded_hp_prop_list {#x#} [] arr \<and> set_mset (mset_nodes x) \<subseteq> \<V> \<and> h = Some (node x)))\<close>
+  \<open>encoded_hp_prop_list_conc = (\<lambda>(\<V>, arr, h) (\<V>', x). \<V> = \<V>' \<and>
+  (case x of None \<Rightarrow> encoded_hp_prop_list \<V>' {#} ([]:: ('a, 'b) hp list) arr \<and> h = None
+  | Some x \<Rightarrow> encoded_hp_prop_list \<V>' {#x#} [] arr \<and> set_mset (mset_nodes x) \<subseteq> set_mset \<V> \<and> h = Some (node x)))\<close>
+
+lemma encoded_hp_prop_list_conc_alt_def:
+  \<open>encoded_hp_prop_list_conc = (\<lambda>(\<V>, arr, h) (\<V>', x). \<V> = \<V>' \<and>
+  (case x of None \<Rightarrow> encoded_hp_prop_list \<V>' {#} ([]:: ('a::linorder, 'b) hp list) arr \<and> h = None
+  | Some x \<Rightarrow> encoded_hp_prop_list \<V>' {#x#} [] arr \<and> h = Some (node x)))\<close>
+  unfolding encoded_hp_prop_list_conc_def encoded_hp_prop_list_def
+  by (auto split: option.splits intro!: ext)
 
 definition encoded_hp_prop_list2_conc
-  :: "'a::linorder set \<times> ('a, 'b) hp_fun \<times> 'a option \<Rightarrow>
-     ('a, 'b) hp list \<Rightarrow> bool"
+  :: "'a::linorder multiset \<times> ('a, 'b) hp_fun \<times> 'a option \<Rightarrow>
+     'a multiset \<times> ('a, 'b) hp list \<Rightarrow> bool"
   where
-  \<open>encoded_hp_prop_list2_conc = (\<lambda>(\<V>, arr, h) x.
-  (encoded_hp_prop_list {#} x arr \<and> set_mset (sum_list (map mset_nodes x)) \<subseteq> \<V> \<and> h = None))\<close>
+  \<open>encoded_hp_prop_list2_conc = (\<lambda>(\<V>, arr, h) (\<V>', x). \<V>' = \<V> \<and>
+  (encoded_hp_prop_list \<V> {#} x arr \<and> set_mset (sum_list (map mset_nodes x)) \<subseteq> set_mset \<V> \<and> h = None))\<close>
+
+lemma encoded_hp_prop_list2_conc_alt_def:
+  \<open>encoded_hp_prop_list2_conc = (\<lambda>(\<V>, arr, h) (\<V>', x). \<V> = \<V>' \<and>
+  (encoded_hp_prop_list \<V> {#} x arr \<and>  h = None))\<close>
+  unfolding encoded_hp_prop_list2_conc_def encoded_hp_prop_list_def
+  by (auto split: option.splits intro!: ext)
 
 lemma encoded_hp_prop_list_update_score:
   fixes h :: \<open>('a, nat) hp\<close> and a arr and hs :: \<open>('a, nat) hp multiset\<close> and x
   defines arr': \<open>arr' \<equiv> hp_update_score a (Some x) arr\<close>
-  assumes enc: \<open>encoded_hp_prop_list (add_mset (Hp a b c) hs) [] arr\<close>
-  shows \<open>encoded_hp_prop_list (add_mset (Hp a x c) hs) []
+  assumes enc: \<open>encoded_hp_prop_list \<V> (add_mset (Hp a b c) hs) [] arr\<close>
+  shows \<open>encoded_hp_prop_list \<V> (add_mset (Hp a x c) hs) []
         arr'\<close>
 proof -
   obtain prevs nxts childs parents scores \<V> where
@@ -706,6 +723,8 @@ proof -
     subgoal
       by (auto simp: find_remove_mset_nodes_full hp_update_score_def)
     subgoal
+      by (auto simp: find_remove_mset_nodes_full hp_update_score_def)
+    subgoal
       apply (auto simp: find_remove_mset_nodes_full hp_update_score_def)
       by (metis hp_child_hp_children_simps2)
     subgoal
@@ -732,17 +751,17 @@ qed
 
 subsubsection \<open>Refinement to Imperative version\<close>
 
-definition hp_insert :: \<open>'a \<Rightarrow> 'b::linorder \<Rightarrow> 'a set \<times> ('a,'b) hp_fun \<times> 'a option \<Rightarrow> ('a set \<times> ('a,'b) hp_fun \<times> 'a option) nres\<close> where
-  \<open>hp_insert = (\<lambda>(i::'a) (w::'b) (\<V>::'a set, arr :: ('a, 'b) hp_fun, h :: 'a option). do {
+definition hp_insert :: \<open>'a \<Rightarrow> 'b::linorder \<Rightarrow> 'a multiset \<times> ('a,'b) hp_fun \<times> 'a option \<Rightarrow> ('a multiset \<times> ('a,'b) hp_fun \<times> 'a option) nres\<close> where
+  \<open>hp_insert = (\<lambda>(i::'a) (w::'b) (\<V>::'a multiset, arr :: ('a, 'b) hp_fun, h :: 'a option). do {
   if h = None then do {
-    ASSERT (i \<in> \<V>);
+    ASSERT (i \<in># \<V>);
     RETURN (\<V>, hp_set_all i None None None None (Some w) arr, Some i)
    } else do {
-    ASSERT (i \<in> \<V>);
+    ASSERT (i \<in># \<V>);
     ASSERT (hp_read_prev i arr = None);
     ASSERT (hp_read_parent i arr = None);
     let (j::'a) = ((the h) :: 'a);
-    ASSERT (j \<in> (\<V>::'a set) \<and> j \<noteq> i);
+    ASSERT (j \<in># \<V> \<and> j \<noteq> i);
     ASSERT (hp_read_score j (arr :: ('a, 'b) hp_fun) \<noteq> None);
     ASSERT (hp_read_prev j arr = None \<and> hp_read_nxt j arr = None \<and> hp_read_parent j arr = None);
     let y = (the (hp_read_score j arr)::'b);
@@ -755,7 +774,7 @@ definition hp_insert :: \<open>'a \<Rightarrow> 'b::linorder \<Rightarrow> 'a se
     }
     else do {
       let child = hp_read_child j arr;
-      ASSERT (child \<noteq> None \<longrightarrow> the child \<in> \<V>);
+      ASSERT (child \<noteq> None \<longrightarrow> the child \<in># \<V>);
       let arr = hp_set_all j None None (Some i) None (Some y) arr;
       let arr = hp_set_all i None child None (Some j) (Some (w::'b)) arr;
       let arr = (if child = None then arr else hp_update_prev (the child) (Some i) arr);
@@ -769,56 +788,56 @@ definition hp_insert :: \<open>'a \<Rightarrow> 'b::linorder \<Rightarrow> 'a se
 lemma hp_insert_spec:
   assumes \<open>encoded_hp_prop_list_conc arr h\<close> and
     \<open>snd h \<noteq> None \<Longrightarrow> i \<notin># mset_nodes (the (snd h))\<close> and
-    \<open>i \<in> fst arr\<close>
+    \<open>i \<in># fst arr\<close>
   shows \<open>hp_insert i w arr \<le> \<Down> {(arr, h). encoded_hp_prop_list_conc arr h}  (ACIDS.mop_hm_insert i w h)\<close>
 proof -
   let ?h = \<open>snd h\<close>
   obtain prevs nxts childs scores parents \<V> where
-    arr: \<open>arr = (\<V>, (prevs, nxts, childs, parents, scores), map_option node ?h)\<close>
+    arr: \<open>arr = (\<V>, (prevs, nxts, childs, parents, scores), map_option node ?h)\<close> 
     by (cases arr; cases ?h) (use assms in \<open>auto simp: encoded_hp_prop_list_conc_def encoded_hp_prop_list_def
         encoded_hp_prop_def\<close>)
 
-  have enc: \<open>encoded_hp_prop {#Hp i w [the h]#}
-    (prevs, nxts(i := None, node (the h) := None), childs(i \<mapsto> node (the h)), parents(node (the h) \<mapsto> i), scores(i \<mapsto> w))\<close> and
-    enc2: \<open>encoded_hp_prop {#Hp (node (the h)) (score (the h)) (Hp i w [] # hps (the h))#}
-   (if hps (the h) = [] then prevs else prevs(node (hd (hps (the h))) \<mapsto> node (Hp i w [])),
-    nxts  (i := None,  node (Hp i w []) := if hps (the h) = [] then None else Some (node (hd (hps (the h))))),
-    childs(i := None)(node (the h) \<mapsto> node (Hp i w [])),
-    (if hps (the h) = [] then parents else parents(node (hd (hps (the h))) := None))(node (Hp i w []) \<mapsto> node (the h)),
-    scores(i \<mapsto> w, node (the h) \<mapsto> score (the h)))\<close> (is ?G)
-    if \<open>h \<noteq> None\<close>
+  have enc: \<open>encoded_hp_prop \<V> {#Hp i w [the ?h]#}
+    (prevs, nxts(i := None, node (the ?h) := None), childs(i \<mapsto> node (the ?h)), parents(node (the ?h) \<mapsto> i), scores(i \<mapsto> w))\<close> and
+    enc2: \<open>encoded_hp_prop \<V> {#Hp (node (the ?h)) (score (the ?h)) (Hp i w [] # hps (the ?h))#}
+   (if hps (the ?h) = [] then prevs else prevs(node (hd (hps (the ?h))) \<mapsto> node (Hp i w [])),
+    nxts  (i := None,  node (Hp i w []) := if hps (the ?h) = [] then None else Some (node (hd (hps (the ?h))))),
+    childs(i := None)(node (the ?h) \<mapsto> node (Hp i w [])),
+    (if hps (the ?h) = [] then parents else parents(node (hd (hps (the ?h))) := None))(node (Hp i w []) \<mapsto> node (the ?h)),
+    scores(i \<mapsto> w, node (the ?h) \<mapsto> score (the ?h)))\<close> (is ?G)
+    if \<open>?h \<noteq> None\<close>
   proof -
-    have \<open>encoded_hp_prop {#the h#} (prevs, nxts, childs, parents, scores)\<close>
+    have \<open>encoded_hp_prop \<V> {#the ?h#} (prevs, nxts, childs, parents, scores)\<close>
       using that assms by (auto simp: encoded_hp_prop_list_conc_def encoded_hp_prop_list_def
         encoded_hp_prop_def arr)
-    then have 0: \<open>encoded_hp_prop {#Hp i w [], the h#}
+    then have 0: \<open>encoded_hp_prop \<V> {#Hp i w [], the ?h#}
       (prevs, nxts(i := None), childs(i := None), parents, scores(i \<mapsto> w))\<close>
-      using encoded_hp_prop_irrelevant[of i \<open>{#the h#}\<close> prevs nxts childs parents scores w] that assms
-      by auto
+      using encoded_hp_prop_irrelevant[of i \<open>{#the ?h#}\<close> \<V> prevs nxts childs parents scores w] that assms
+      by (auto simp: arr)
     from encoded_hp_prop_link[OF this]
-    show \<open>encoded_hp_prop {#Hp i w [the h]#}
-      (prevs, nxts(i := None, node (the h) := None), childs(i \<mapsto> node (the h)), parents(node (the h) \<mapsto> i), scores(i \<mapsto> w))\<close>
+    show \<open>encoded_hp_prop \<V> {#Hp i w [the ?h]#}
+      (prevs, nxts(i := None, node (the ?h) := None), childs(i \<mapsto> node (the ?h)), parents(node (the ?h) \<mapsto> i), scores(i \<mapsto> w))\<close>
       by auto
-    from 0 have \<open>encoded_hp_prop {#Hp (node (the h)) (score (the h)) (hps (the h)), Hp i w []#}
+    from 0 have \<open>encoded_hp_prop \<V> {#Hp (node (the ?h)) (score (the ?h)) (hps (the ?h)), Hp i w []#}
       (prevs, nxts(i := None), childs(i := None), parents, scores(i \<mapsto> w))\<close>
-      by (cases \<open>the h\<close>) (auto simp: add_mset_commute)
+      by (cases \<open>the ?h\<close>) (auto simp: add_mset_commute)
     from encoded_hp_prop_link[OF this]
     show ?G .
   qed
   have prev_parent_i:
-    \<open>h \<noteq> None \<Longrightarrow> hp_read_prev i (prevs, nxts, childs, parents, scores) = None\<close>
-    \<open>h \<noteq> None \<Longrightarrow> hp_read_parent i (prevs, nxts, childs, parents, scores) = None\<close>
+    \<open>?h \<noteq> None \<Longrightarrow> hp_read_prev i (prevs, nxts, childs, parents, scores) = None\<close>
+    \<open>?h \<noteq> None \<Longrightarrow> hp_read_parent i (prevs, nxts, childs, parents, scores) = None\<close>
     using assms unfolding encoded_hp_prop_list_conc_def
     by (force simp: arr encoded_hp_prop_def empty_outside_alt_def dest!: multi_member_split[of i])+
-  have 1: \<open>h \<noteq> None \<Longrightarrow> hps (the h) \<noteq> [] \<Longrightarrow> i \<noteq> node (hd (hps (the h)))\<close>
-    using assms by (cases \<open>the h\<close>; cases \<open>hps (the h)\<close>; cases h) auto
-  have [simp]: \<open>encoded_hp_prop {#Hp x1a x2 x3#} (prevs, nxts, childs, parents, scores) \<Longrightarrow> scores x1a = Some x2\<close>
-    \<open>encoded_hp_prop {#Hp x1a x2 x3#} (prevs, nxts, childs, parents, scores) \<Longrightarrow> parents x1a = None\<close>
-    \<open>encoded_hp_prop {#Hp x1a x2 x3#} (prevs, nxts, childs, parents, scores) \<Longrightarrow> childs x1a = map_option node (option_hd x3)\<close> for x1a x2 x3
+  have 1: \<open>?h \<noteq> None \<Longrightarrow> hps (the ?h) \<noteq> [] \<Longrightarrow> i \<noteq> node (hd (hps (the ?h)))\<close>
+    using assms by (cases \<open>the ?h\<close>; cases \<open>hps (the ?h)\<close>; cases h) auto
+  have [simp]: \<open>encoded_hp_prop \<V> {#Hp x1a x2 x3#} (prevs, nxts, childs, parents, scores) \<Longrightarrow> scores x1a = Some x2\<close>
+    \<open>encoded_hp_prop \<V> {#Hp x1a x2 x3#} (prevs, nxts, childs, parents, scores) \<Longrightarrow> parents x1a = None\<close>
+    \<open>encoded_hp_prop \<V> {#Hp x1a x2 x3#} (prevs, nxts, childs, parents, scores) \<Longrightarrow> childs x1a = map_option node (option_hd x3)\<close> for x1a x2 x3
     by (auto simp: encoded_hp_prop_def)
   show ?thesis
     using assms
-    unfolding hp_insert_def arr prod.simps
+    unfolding hp_insert_def arr prod.simps ACIDS.mop_hm_insert_def
     apply refine_vcg
     subgoal
       by auto
@@ -837,10 +856,10 @@ proof -
       by (auto simp: encoded_hp_prop_list_conc_def encoded_hp_prop_list_def hp_set_all_def
         split: option.splits prod.splits)
     subgoal
-      by (cases \<open>the h\<close>) (auto simp: encoded_hp_prop_list_conc_def encoded_hp_prop_list_def hp_set_all_def
+      by (cases \<open>the ?h\<close>) (auto simp: encoded_hp_prop_list_conc_def encoded_hp_prop_list_def hp_set_all_def
         split: option.splits prod.splits)
     subgoal
-      by (cases \<open>the h\<close>) (auto simp: encoded_hp_prop_list_conc_def encoded_hp_prop_list_def hp_set_all_def
+      by (cases \<open>the ?h\<close>) (auto simp: encoded_hp_prop_list_conc_def encoded_hp_prop_list_def hp_set_all_def
         split: option.splits prod.splits)
     subgoal
       by (auto simp: encoded_hp_prop_list_conc_def encoded_hp_prop_list_def hp_set_all_def
@@ -850,25 +869,26 @@ proof -
         split: option.splits prod.splits)
     subgoal
       using enc
-      by (cases h, simp; cases \<open>the h\<close>)
+      by (cases h, simp; cases \<open>the ?h\<close>)
         (auto simp: hp_set_all_def encoded_hp_prop_list_conc_def fun_upd_idem hp_update_parents_def)
     subgoal
       using enc
-      by (cases h, simp; cases \<open>the h\<close>)
-        (auto simp: hp_set_all_def encoded_hp_prop_list_conc_def fun_upd_idem hp_update_parents_def)
+      by (cases h, simp; cases \<open>the ?h\<close>; cases \<open>hps (the ?h)\<close>; cases \<open>hd (hps (the ?h))\<close>)
+        (auto simp: hp_set_all_def encoded_hp_prop_list_conc_def fun_upd_idem hp_update_parents_def
+        arr)
     subgoal
       using enc2 1
-      by (cases h, simp; cases \<open>the h\<close>)
+      by (cases h, simp; cases \<open>the ?h\<close>)
         (auto simp: hp_set_all_def encoded_hp_prop_list_conc_def fun_upd_idem hp_update_prev_def
           fun_upd_twist hp_update_parents_def)
      done
 qed
 
-definition hp_link :: \<open>'a \<Rightarrow> 'a \<Rightarrow> 'a set \<times> ('a,'b::order) hp_fun \<times> 'a option \<Rightarrow> (('a set \<times> ('a,'b) hp_fun \<times> 'a option) \<times> 'a) nres\<close> where
-  \<open>hp_link = (\<lambda>(i::'a) j (\<V>::'a set, arr :: ('a, 'b) hp_fun, h :: 'a option). do {
+definition hp_link :: \<open>'a \<Rightarrow> 'a \<Rightarrow> 'a multiset \<times> ('a,'b::order) hp_fun \<times> 'a option \<Rightarrow> (('a multiset \<times> ('a,'b) hp_fun \<times> 'a option) \<times> 'a) nres\<close> where
+  \<open>hp_link = (\<lambda>(i::'a) j (\<V>::'a multiset, arr :: ('a, 'b) hp_fun, h :: 'a option). do {
     ASSERT (i \<noteq> j);
-    ASSERT (i \<in> \<V>);
-    ASSERT (j \<in> \<V>);
+    ASSERT (i \<in># \<V>);
+    ASSERT (j \<in># \<V>);
     ASSERT (hp_read_score i arr \<noteq> None);
     ASSERT (hp_read_score j arr \<noteq> None);
     let x = (the (hp_read_score i arr)::'b);
@@ -887,11 +907,11 @@ definition hp_link :: \<open>'a \<Rightarrow> 'a \<Rightarrow> 'a set \<times> (
       @ (if prev \<noteq> None then [the prev] else [])
       @ (if nxt \<noteq> None then [the nxt] else []))
       );
-    ASSERT (ch \<in> \<V>);
-    ASSERT (parent \<in> \<V>);
-    ASSERT (child \<noteq> None \<longrightarrow> the child \<in> \<V>);
-    ASSERT (nxt \<noteq> None \<longrightarrow> the nxt \<in> \<V>);
-    ASSERT (prev \<noteq> None \<longrightarrow> the prev \<in> \<V>);
+    ASSERT (ch \<in># \<V>);
+    ASSERT (parent \<in># \<V>);
+    ASSERT (child \<noteq> None \<longrightarrow> the child \<in># \<V>);
+    ASSERT (nxt \<noteq> None \<longrightarrow> the nxt \<in># \<V>);
+    ASSERT (prev \<noteq> None \<longrightarrow> the prev \<in># \<V>);
     let arr = hp_set_all parent prev nxt (Some ch) None (Some (w\<^sub>p::'b)) (arr::('a, 'b) hp_fun);
     let arr = hp_set_all ch None child child\<^sub>c\<^sub>h (Some parent) (Some (w\<^sub>c\<^sub>h::'b)) (arr::('a, 'b) hp_fun);
     let arr = (if child = None then arr else hp_update_prev (the child) (Some ch) arr);
@@ -906,16 +926,17 @@ lemma fun_upd_twist2: "a \<noteq> c \<Longrightarrow> a \<noteq> e \<Longrightar
   by auto
 
 lemma hp_link:
-  assumes enc: \<open>encoded_hp_prop_list2_conc arr (xs @ x # y # ys)\<close> and
+  assumes enc: \<open>encoded_hp_prop_list2_conc arr (\<V>', xs @ x # y # ys)\<close> and
     \<open>i = node x\<close> and
     \<open>j = node y\<close>
-  shows \<open>hp_link i j arr \<le> SPEC (\<lambda>(arr, n). encoded_hp_prop_list2_conc arr (xs @ ACIDS.link x y # ys) \<and>
+  shows \<open>hp_link i j arr \<le> SPEC (\<lambda>(arr, n). encoded_hp_prop_list2_conc arr (\<V>', xs @ ACIDS.link x y # ys) \<and>
     n = node (ACIDS.link x y))\<close>
 proof -
   obtain prevs nxts childs parents scores \<V> where
     arr: \<open>arr = (\<V>, (prevs, nxts, childs, parents, scores), None)\<close> and
     dist: \<open>distinct_mset (\<Sum>\<^sub># (mset_nodes `# (mset (xs @ x # y # ys))))\<close> and
-    \<V>: \<open>set_mset (sum_list (map mset_nodes (xs @ x # y # ys))) \<subseteq> \<V>\<close>
+    \<V>: \<open>set_mset (sum_list (map mset_nodes (xs @ x # y # ys))) \<subseteq> set_mset \<V>\<close> and
+    \<V>'[simp]: \<open>\<V>' = \<V>\<close>
     by (cases arr) (use assms in \<open>auto simp: ac_simps encoded_hp_prop_list2_conc_def encoded_hp_prop_list_def
         encoded_hp_prop_def\<close>)
 
@@ -1001,22 +1022,22 @@ proof -
        (auto split: if_splits)
   have if_pair: \<open>(if a then (b, c) else (d,f)) = (if a then b else d, if a then c else f)\<close> for a b c d f
     by auto
-  have enc0: \<open>encoded_hp_prop_list {#} (xs @ [Hp (node x) (score x) (hps x), Hp (node y) (score y) (hps y)] @ ys) (prevs, nxts, childs, parents, scores)\<close>
+  have enc0: \<open>encoded_hp_prop_list \<V> {#} (xs @ [Hp (node x) (score x) (hps x), Hp (node y) (score y) (hps y)] @ ys) (prevs, nxts, childs, parents, scores)\<close>
     using enc unfolding x y by (auto simp: encoded_hp_prop_list2_conc_def arr)
-  then have H: \<open>fst x1= \<V> \<Longrightarrow> snd (snd x1) = None\<Longrightarrow> encoded_hp_prop_list2_conc x1 (xs @ ACIDS.link x y # ys) \<longleftrightarrow>
-    encoded_hp_prop_list {#} (xs @ ACIDS.link x y # ys) (fst (snd x1))\<close> for x1
+  then have H: \<open>fst x1= \<V> \<Longrightarrow> snd (snd x1) = None\<Longrightarrow> encoded_hp_prop_list2_conc x1 (\<V>', xs @ ACIDS.link x y # ys) \<longleftrightarrow>
+    encoded_hp_prop_list \<V> {#} (xs @ ACIDS.link x y # ys) (fst (snd x1))\<close> for x1
     using dist \<V> unfolding x y
     by (cases x1)
       (simp add: encoded_hp_prop_list2_conc_def)
   have KK [intro!]: \<open>ch\<^sub>x \<noteq> [] \<Longrightarrow> ys \<noteq> [] \<Longrightarrow> node (hd ch\<^sub>x) \<noteq> node (hd ys)\<close>
     using dist2 sc' by simp
 
-  have subs: \<open>set_mset (sum_list (map mset_nodes (xs @ Hp i w\<^sub>x ch\<^sub>x # Hp j w\<^sub>y ch\<^sub>y # ys))) \<subseteq> \<V>\<close>
+  have subs: \<open>set_mset (sum_list (map mset_nodes (xs @ Hp i w\<^sub>x ch\<^sub>x # Hp j w\<^sub>y ch\<^sub>y # ys))) \<subseteq> set_mset \<V>\<close>
     using assms(1) sc'(7,3) unfolding encoded_hp_prop_list2_conc_def x y arr prod.simps
       encoded_hp_prop_list_def
     by (clarsimp_all simp: encoded_hp_prop_list_def)
-  then have childs_i: \<open>childs i \<noteq> None \<Longrightarrow> the (childs i) \<in> \<V>\<close>
-    \<open>prevs i \<noteq> None \<Longrightarrow> the (prevs i) \<in> \<V>\<close>
+  then have childs_i: \<open>childs i \<noteq> None \<Longrightarrow> the (childs i) \<in># \<V>\<close>
+    \<open>prevs i \<noteq> None \<Longrightarrow> the (prevs i) \<in># \<V>\<close>
     using sc'(7,3) unfolding encoded_hp_prop_list2_conc_def x y arr prod.simps
       encoded_hp_prop_list_def
     apply (clarsimp_all simp: encoded_hp_prop_list_def)
@@ -1024,8 +1045,8 @@ proof -
     by (metis \<V> dist distinct_mset_add hp_next_children_None_notin hp_next_children_last
       list.discI map_append option_hd_Some_hd option_last_Nil option_last_Some_iff(2)
       subset_eq sum_image_mset_sum_map sum_list_append)
-  have childs_j: \<open>childs j \<noteq> None \<Longrightarrow> the (childs j) \<in> \<V>\<close>
-    \<open>nxts j \<noteq> None \<Longrightarrow> the (nxts j) \<in> \<V>\<close>
+  have childs_j: \<open>childs j \<noteq> None \<Longrightarrow> the (childs j) \<in># \<V>\<close>
+    \<open>nxts j \<noteq> None \<Longrightarrow> the (nxts j) \<in># \<V>\<close>
     using subs sc'(6,8) unfolding encoded_hp_prop_list2_conc_def x y arr prod.simps
     apply (clarsimp_all simp: encoded_hp_prop_list_def)
     apply (metis node_hd_in_sum option.sel subsetD)
@@ -1061,7 +1082,7 @@ proof -
         apply (solves simp)
         using p(1-12) p(19)[symmetric] dist2 \<V>
         apply (solves simp)
-        apply (subst arg_cong2[THEN iffD1, of _ _ _ _ \<open>encoded_hp_prop_list {#}\<close>, OF _ _ encoded_hp_prop_list_link[of \<open>{#}\<close> xs \<open>node x\<close> \<open>score x\<close> \<open>hps x\<close> \<open>node y\<close> \<open>score y\<close> \<open>hps y\<close> ys
+        apply (subst arg_cong2[THEN iffD1, of _ _ _ _ \<open>encoded_hp_prop_list \<V> {#}\<close>, OF _ _ encoded_hp_prop_list_link[of \<V> \<open>{#}\<close> xs \<open>node x\<close> \<open>score x\<close> \<open>hps x\<close> \<open>node y\<close> \<open>score y\<close> \<open>hps y\<close> ys
           prevs nxts childs parents scores, OF enc0]])
         subgoal
           using sc' p(1-12) p(19)[symmetric] dist2 \<V>
@@ -1194,7 +1215,7 @@ proof -
         apply simp
         using p(1-12) p(19)[symmetric] dist2 \<V>
         apply simp
-        apply (subst arg_cong2[THEN iffD1, of _ _ _ _ \<open>encoded_hp_prop_list {#}\<close>, OF _ _ encoded_hp_prop_list_link2[of \<open>{#}\<close> xs \<open>node x\<close> \<open>score x\<close> \<open>hps x\<close> \<open>node y\<close> \<open>score y\<close> \<open>hps y\<close> ys
+        apply (subst arg_cong2[THEN iffD1, of _ _ _ _ \<open>encoded_hp_prop_list \<V> {#}\<close>, OF _ _ encoded_hp_prop_list_link2[of \<V> \<open>{#}\<close> xs \<open>node x\<close> \<open>score x\<close> \<open>hps x\<close> \<open>node y\<close> \<open>score y\<close> \<open>hps y\<close> ys
           prevs nxts childs parents scores, OF enc0]])
         subgoal
           using sc' p(1-12) p(19)[symmetric] dist2 \<V>
@@ -1327,18 +1348,18 @@ text \<open>In an imperative setting use the two pass approaches is better than 
 
 The \<^term>\<open>e::nat\<close> of the loop is a dummy counter.\<close>
 definition vsids_pass\<^sub>1 where
-  \<open>vsids_pass\<^sub>1 = (\<lambda>(\<V>::'a set, arr :: ('a, 'b::order) hp_fun, h :: 'a option) (j::'a). do {
+  \<open>vsids_pass\<^sub>1 = (\<lambda>(\<V>::'a multiset, arr :: ('a, 'b::order) hp_fun, h :: 'a option) (j::'a). do {
   ((\<V>, arr, h), j, _, n) \<leftarrow> WHILE\<^sub>T(\<lambda>((\<V>, arr, h), j, e, n). j \<noteq> None)
   (\<lambda>((\<V>, arr, h), j, e::nat, n). do {
     if j = None then RETURN ((\<V>, arr, h), None, e, n)
     else do {
     let j = the j;
-    ASSERT (j \<in> \<V>);
+    ASSERT (j \<in># \<V>);
     let nxt = hp_read_nxt j arr;
     if nxt = None then RETURN ((\<V>, arr, h), nxt, e+1, j)
     else do {
       ASSERT (nxt \<noteq> None);
-      ASSERT (the nxt \<in> \<V>);
+      ASSERT (the nxt \<in># \<V>);
       let nnxt = hp_read_nxt (the nxt) arr;
       ((\<V>, arr, h), n) \<leftarrow> hp_link j (the nxt) (\<V>, arr, h);
       RETURN ((\<V>, arr, h), nnxt, e+2, n)
@@ -1350,18 +1371,19 @@ definition vsids_pass\<^sub>1 where
 
 
 lemma vsids_pass\<^sub>1:
-  fixes arr :: \<open>'a::linorder set \<times> ('a, nat) hp_fun \<times> 'a option\<close>
-  assumes \<open>encoded_hp_prop_list2_conc arr xs\<close> and \<open>xs \<noteq> []\<close> and \<open>j = node (hd xs)\<close>
-  shows \<open>vsids_pass\<^sub>1 arr j \<le> SPEC(\<lambda>(arr, j). encoded_hp_prop_list2_conc arr (ACIDS.pass\<^sub>1 xs) \<and> j = node (last (ACIDS.pass\<^sub>1 xs)))\<close>
+  fixes arr :: \<open>'a::linorder multiset \<times> ('a, nat) hp_fun \<times> 'a option\<close>
+  assumes \<open>encoded_hp_prop_list2_conc arr (\<V>', xs)\<close> and \<open>xs \<noteq> []\<close> and \<open>j = node (hd xs)\<close>
+  shows \<open>vsids_pass\<^sub>1 arr j \<le> SPEC(\<lambda>(arr, j). encoded_hp_prop_list2_conc arr (\<V>', ACIDS.pass\<^sub>1 xs) \<and> j = node (last (ACIDS.pass\<^sub>1 xs)))\<close>
 proof -
   obtain prevs nxts childs scores \<V> where
     arr: \<open>arr = (\<V>, (prevs, nxts, childs, scores), None)\<close> and
     dist: \<open>distinct_mset (\<Sum>\<^sub># (mset_nodes `# (mset (xs))))\<close> and
-    \<V>: \<open>set_mset (sum_list (map mset_nodes xs)) \<subseteq> \<V>\<close>
+    \<V>: \<open>set_mset (sum_list (map mset_nodes xs)) \<subseteq> set_mset \<V>\<close> and
+    [simp]: \<open>\<V>' = \<V>\<close>
     by (cases arr) (use assms in \<open>auto simp: ac_simps encoded_hp_prop_list2_conc_def encoded_hp_prop_list_def
         encoded_hp_prop_def\<close>)
   define I where \<open>I \<equiv> (\<lambda>(arr, nnxt::'a option, e, k).
-    encoded_hp_prop_list2_conc arr (ACIDS.pass\<^sub>1(take e xs) @ drop e xs) \<and> nnxt = map_option node (option_hd (drop (e) xs)) \<and>
+    encoded_hp_prop_list2_conc arr (\<V>, ACIDS.pass\<^sub>1(take e xs) @ drop e xs) \<and> nnxt = map_option node (option_hd (drop (e) xs)) \<and>
     e \<le> (length xs) \<and> (nnxt = None \<longleftrightarrow> e = length xs) \<and> (nnxt \<noteq> None \<longrightarrow> even e) \<and>
     k = (if e=0 then j else node (last (ACIDS.pass\<^sub>1(take e xs)))))\<close>
   have I0: \<open>I ((\<V>, (prevs, nxts, childs, scores), None), Some j, 0, j)\<close>
@@ -1392,7 +1414,7 @@ proof -
   qed
 
   have link_pre1: \<open>encoded_hp_prop_list2_conc (x1, x1a, x2a)
-    (ACIDS.pass\<^sub>1 (take x2b xs) @
+    (\<V>', ACIDS.pass\<^sub>1 (take x2b xs) @
     xs!x2b # xs!(Suc x2b) # drop (x2b+2) xs)\<close> (is ?H1) and
     link_pre2: \<open>the x1b = node (xs ! x2b)\<close>  (is ?H2) and
     link_pre3: \<open>the (hp_read_nxt (the x1b) x1a) = node (xs ! Suc x2b)\<close> (is ?H3)
@@ -1407,11 +1429,11 @@ proof -
       nxt: \<open>hp_read_nxt (the x1b) x1a \<noteq> None\<close>
     for s a b x1 x2 x1a x2a x1b x2b j x2b'
   proof -
-    have \<open>encoded_hp_prop_list {#} (ACIDS.pass\<^sub>1 (take x2b xs) @ drop x2b xs) x1a\<close>
+    have \<open>encoded_hp_prop_list x1 {#} (ACIDS.pass\<^sub>1 (take x2b xs) @ drop x2b xs) x1a\<close>
       \<open>x2b < length xs\<close>
       \<open>x1b = Some (node (hd (drop x2b xs)))\<close>
       using that
-      by (auto simp: I_def encoded_hp_prop_list2_conc_def)
+      by (auto simp: I_def encoded_hp_prop_list2_conc_def arr)
     then have \<open>drop x2b xs \<noteq> []\<close> \<open>tl (drop x2b xs) \<noteq> []\<close> \<open>Suc x2b < length xs\<close> \<open>the x1b = node (xs ! x2b)\<close>
       \<open>the (hp_read_nxt (the x1b) x1a) = node (xs ! Suc x2b)\<close>
       using nxt unfolding s apply -
@@ -1451,7 +1473,7 @@ proof -
         \<open>b = (nxt, k')\<close>
         \<open>k' = (k, j)\<close>
         \<open>x1a = (x2a, x1b)\<close>
-        \<open>arr2 = (\<V>', x1a)\<close>
+        \<open>arr2 = (\<V>'', x1a)\<close>
         \<open>linkedn = (linked, n)\<close>
         \<open>x1d = (x2d, xe)\<close>
         \<open>linked = (x2c, x1d)\<close> and
@@ -1461,11 +1483,11 @@ proof -
       linkedn: \<open>case linkedn of
       (arr, n) \<Rightarrow>
       encoded_hp_prop_list2_conc arr
-      (ACIDS.pass\<^sub>1 (take k xs) @ ACIDS.link (xs ! k) (xs ! Suc k) # drop (k + 2) xs) \<and>
+      (\<V>', ACIDS.pass\<^sub>1 (take k xs) @ ACIDS.link (xs ! k) (xs ! Suc k) # drop (k + 2) xs) \<and>
       n = node (ACIDS.link (xs ! k) (xs ! Suc k))\<close>
-    for s arr2 b \<V>' x1a x2a x1b nxt k linkedn linked n x2c x1d x2d xe j k'
+    for s arr2 b x1a x2a x1b nxt k linkedn linked n x2c x1d x2d xe j k' \<V>''
   proof -
-    have enc: \<open>encoded_hp_prop_list {#} (ACIDS.pass\<^sub>1 (take k xs) @ drop k xs) x2a\<close>
+    have enc: \<open>encoded_hp_prop_list \<V>' {#} (ACIDS.pass\<^sub>1 (take k xs) @ drop k xs) x2a\<close>
       \<open>k < length xs\<close>
       \<open>nxt = Some (node (hd (drop k xs)))\<close> and
       dist: \<open>distinct_mset (\<Sum>\<^sub># (mset_nodes `# (mset (ACIDS.pass\<^sub>1 (take k xs) @ drop k xs))))\<close>
@@ -1549,15 +1571,15 @@ proof -
 qed
 
 definition vsids_pass\<^sub>2 where
-  \<open>vsids_pass\<^sub>2 = (\<lambda>(\<V>::'a set, arr :: ('a, 'b::order) hp_fun, h :: 'a option) (j::'a). do {
-  ASSERT (j \<in> \<V>);
+  \<open>vsids_pass\<^sub>2 = (\<lambda>(\<V>::'a multiset, arr :: ('a, 'b::order) hp_fun, h :: 'a option) (j::'a). do {
+  ASSERT (j \<in># \<V>);
   let nxt = hp_read_prev j arr;
   ((\<V>, arr, h), j, leader, _) \<leftarrow> WHILE\<^sub>T(\<lambda>((\<V>, arr, h), j, leader, e). j \<noteq> None)
   (\<lambda>((\<V>, arr, h), j, leader, e::nat). do {
     if j = None then RETURN ((\<V>, arr, h), None, leader, e)
     else do {
       let j = the j;
-      ASSERT (j \<in> \<V>);
+      ASSERT (j \<in># \<V>);
       let nnxt = hp_read_prev j arr;
       ((\<V>, arr, h), n) \<leftarrow> hp_link j leader (\<V>, arr, h);
       RETURN ((\<V>, arr, h), nnxt, n, e+1)
@@ -1567,15 +1589,17 @@ definition vsids_pass\<^sub>2 where
   RETURN (\<V>, arr, Some leader)
   })\<close>
 
+
 lemma vsids_pass\<^sub>2:
-  fixes arr :: \<open>'a::linorder set \<times> ('a, nat) hp_fun \<times> 'a option\<close>
-  assumes \<open>encoded_hp_prop_list2_conc arr xs\<close> and \<open>xs \<noteq> []\<close> and \<open>j = node (last xs)\<close>
-  shows \<open>vsids_pass\<^sub>2 arr j \<le> SPEC(\<lambda>(arr). encoded_hp_prop_list_conc arr (ACIDS.pass\<^sub>2 xs))\<close>
+  fixes arr :: \<open>'a::linorder multiset \<times> ('a, nat) hp_fun \<times> 'a option\<close>
+  assumes \<open>encoded_hp_prop_list2_conc arr (\<V>', xs)\<close> and \<open>xs \<noteq> []\<close> and \<open>j = node (last xs)\<close>
+  shows \<open>vsids_pass\<^sub>2 arr j \<le> SPEC(\<lambda>(arr). encoded_hp_prop_list_conc arr (\<V>', ACIDS.pass\<^sub>2 xs))\<close>
 proof -
   obtain prevs nxts childs scores \<V> where
     arr: \<open>arr = (\<V>, (prevs, nxts, childs, scores), None)\<close> and
     dist: \<open>distinct_mset (\<Sum>\<^sub># (mset_nodes `# (mset (xs))))\<close> and
-    \<V>: \<open>set_mset (sum_list (map mset_nodes xs)) \<subseteq> \<V>\<close>
+    \<V>: \<open>set_mset (sum_list (map mset_nodes xs)) \<subseteq> set_mset \<V>\<close> and
+    [simp]: \<open>\<V>' = \<V>\<close>
     by (cases arr) (use assms in \<open>auto simp: ac_simps encoded_hp_prop_list2_conc_def encoded_hp_prop_list_def
         encoded_hp_prop_def\<close>)
   have prevs_lastxs: \<open>prevs (node (last xs)) = map_option node (option_last (butlast xs))\<close>
@@ -1584,16 +1608,16 @@ proof -
      (auto simp: encoded_hp_prop_list2_conc_def encoded_hp_prop_list_def arr)
 
   define I where \<open>I \<equiv> (\<lambda>(arr, nnxt::'a option, leader, e'). let e = length xs - e' in
-    encoded_hp_prop_list2_conc arr (take e xs @ [the (ACIDS.pass\<^sub>2 (drop e xs))]) \<and> nnxt = map_option node (option_last (take e xs)) \<and>
+    encoded_hp_prop_list2_conc arr (\<V>, take e xs @ [the (ACIDS.pass\<^sub>2 (drop e xs))]) \<and> nnxt = map_option node (option_last (take e xs)) \<and>
     leader = node (the (ACIDS.pass\<^sub>2 (drop e xs))) \<and>
     e \<le> (length xs) \<and> (nnxt = None \<longleftrightarrow> e = 0) \<and> e' > 0)\<close>
   have I0: \<open>I ((\<V>, (prevs, nxts, childs, scores), None), hp_read_prev j (prevs, nxts, childs, scores), j, 1)\<close>
     using assms prevs_lastxs unfolding I_def prod.simps Let_def
     by (auto simp: arr butlast_Nil_iff)
-  have j\<V>: \<open>j \<in> \<V>\<close>
+  have j\<V>: \<open>j \<in># \<V>\<close>
     using assms by (cases xs rule: rev_cases) (auto simp: encoded_hp_prop_list2_conc_def arr)
   have links_pre1: \<open>encoded_hp_prop_list2_conc (\<V>', arr', h')
-    (take (length xs - Suc e) xs @
+    (\<V>, take (length xs - Suc e) xs @
     xs ! (length xs - Suc e) #
     the (ACIDS.pass\<^sub>2 (drop (length xs - e) xs)) # [])\<close> (is ?H1) and
     links_pre2: \<open>the x1b = node (xs ! (length xs - Suc e))\<close> (is ?H2) and
@@ -1648,7 +1672,7 @@ proof -
       \<open>case linkedn of
       (arr, n) \<Rightarrow>
       encoded_hp_prop_list2_conc arr
-      (take (length xs - Suc e) xs @
+      (\<V>, take (length xs - Suc e) xs @
       [ACIDS.link (xs ! (length xs - Suc e)) (the (ACIDS.pass\<^sub>2 (drop (length xs - e) xs)))]) \<and>
       n =
       node
@@ -1707,13 +1731,13 @@ definition merge_pairs where
 
 
 lemma vsids_merge_pairs:
-  fixes arr :: \<open>'a::linorder set \<times> ('a, nat) hp_fun \<times> 'a option\<close>
-  assumes \<open>encoded_hp_prop_list2_conc arr xs\<close> and \<open>xs \<noteq> []\<close> and \<open>j = node (hd xs)\<close>
-  shows \<open>merge_pairs arr j \<le> SPEC(\<lambda>(arr). encoded_hp_prop_list_conc arr (ACIDS.merge_pairs xs))\<close>
+  fixes arr :: \<open>'a::linorder multiset \<times> ('a, nat) hp_fun \<times> 'a option\<close>
+  assumes \<open>encoded_hp_prop_list2_conc arr (\<V>', xs)\<close> and \<open>xs \<noteq> []\<close> and \<open>j = node (hd xs)\<close>
+  shows \<open>merge_pairs arr j \<le> SPEC(\<lambda>(arr). encoded_hp_prop_list_conc arr (\<V>', ACIDS.merge_pairs xs))\<close>
 proof -
   show ?thesis
     unfolding merge_pairs_def
-    apply (refine_vcg vsids_pass\<^sub>1 vsids_pass\<^sub>2[of _ "ACIDS.pass\<^sub>1 xs"])
+    apply (refine_vcg vsids_pass\<^sub>1 vsids_pass\<^sub>2[of _ \<V>' "ACIDS.pass\<^sub>1 xs"])
     apply (rule assms)+
     subgoal by auto
     subgoal using assms by (cases xs rule: ACIDS.pass\<^sub>1.cases) auto
@@ -1727,14 +1751,14 @@ definition hp_update_child where
   \<open>hp_update_child i nxt = (\<lambda>(prevs, nxts, childs, scores). (prevs, nxts, childs(i:=nxt), scores))\<close>
 
 definition vsids_pop_min :: \<open>_\<close> where
-  \<open>vsids_pop_min = (\<lambda>(\<V>::'a set, arr :: ('a, 'b::order) hp_fun, h :: 'a option). do {
+  \<open>vsids_pop_min = (\<lambda>(\<V>::'a multiset, arr :: ('a, 'b::order) hp_fun, h :: 'a option). do {
   if h = None then RETURN (None, (\<V>, arr, h))
   else do {
-      ASSERT (the h \<in> \<V>);
+      ASSERT (the h \<in># \<V>);
       let j = hp_read_child (the h) arr;
       if j = None then RETURN (h, (\<V>, arr, None))
       else do {
-        ASSERT (the j \<in> \<V>);
+        ASSERT (the j \<in># \<V>);
         let arr = hp_update_prev (the h) None arr;
         let arr = hp_update_child (the h) None arr;
         let arr = hp_update_parents (the j) None arr;
@@ -1748,13 +1772,13 @@ lemma node_remove_key_itself_iff[simp]: \<open>remove_key (y) z \<noteq> None \<
   by (cases z) auto
 
 lemma vsids_pop_min:
-  fixes arr :: \<open>'a::linorder set \<times> ('a, nat) hp_fun \<times> 'a option\<close>
-  assumes \<open>encoded_hp_prop_list_conc arr h\<close>
-  shows \<open>vsids_pop_min arr \<le> SPEC(\<lambda>(j, arr). j = (if h = None then None else Some (get_min2 h)) \<and> encoded_hp_prop_list_conc arr (ACIDS.del_min h))\<close>
+  fixes arr :: \<open>'a::linorder multiset \<times> ('a, nat) hp_fun \<times> 'a option\<close>
+  assumes \<open>encoded_hp_prop_list_conc arr (\<V>, h)\<close>
+  shows \<open>vsids_pop_min arr \<le> SPEC(\<lambda>(j, arr). j = (if h = None then None else Some (get_min2 h)) \<and> encoded_hp_prop_list_conc arr (\<V>, ACIDS.del_min h))\<close>
 proof -
   show ?thesis
     unfolding vsids_pop_min_def
-    apply (refine_vcg vsids_merge_pairs[of _ \<open>case the h of Hp _ _ child \<Rightarrow> child\<close>])
+    apply (refine_vcg vsids_merge_pairs[of _ \<V> \<open>case the h of Hp _ _ child \<Rightarrow> child\<close>])
     subgoal using assms by (cases h) (auto simp: encoded_hp_prop_list_conc_def)
     subgoal using assms by (auto simp: encoded_hp_prop_list_conc_def split: option.splits)
     subgoal using assms by (auto simp: encoded_hp_prop_list_conc_def split: option.splits)
@@ -1763,7 +1787,7 @@ proof -
       get_min2_alt_def split: option.splits)
     subgoal using assms by (cases \<open>the h\<close>) (auto simp: encoded_hp_prop_list_conc_def encoded_hp_prop_def
       get_min2_alt_def split: option.splits)
-    subgoal using assms encoded_hp_prop_list_remove_min[of \<open>node (the h)\<close> \<open>score (the h)\<close> \<open>hps (the h)\<close> \<open>{#}\<close>
+    subgoal using assms encoded_hp_prop_list_remove_min[of \<V> \<open>node (the h)\<close> \<open>score (the h)\<close> \<open>hps (the h)\<close> \<open>{#}\<close>
       \<open>fst (fst (snd arr))\<close> \<open>(fst o snd) (fst (snd arr))\<close> \<open>(fst o snd o snd) (fst (snd arr))\<close>
       \<open>(fst o snd o snd o snd) (fst (snd arr))\<close>
       \<open>(snd o snd o snd o snd) (fst (snd arr))\<close>]
@@ -1897,15 +1921,15 @@ lemma encoded_hp_prop_list_remove_find:
   defines \<open>arr\<^sub>3 \<equiv> (if hp_next a h = None then arr\<^sub>2 else hp_update_prev (node (the (hp_next a h))) (map_option node (hp_prev a h)) arr\<^sub>2)\<close>
   defines \<open>arr\<^sub>4 \<equiv> (if hp_next a h = None then arr\<^sub>3 else hp_update_parents (node (the (hp_next a h))) (map_option node (hp_parent a h)) arr\<^sub>3)\<close>
   defines \<open>arr' \<equiv> hp_update_parents a None (hp_update_prev a None (hp_update_nxt a None arr\<^sub>4))\<close>
-  assumes enc: \<open>encoded_hp_prop_list (add_mset h {#}) [] arr\<close>
-  shows \<open>encoded_hp_prop_list ((if remove_key a h = None then {#} else {#the (remove_key a h)#}) +
+  assumes enc: \<open>encoded_hp_prop_list \<V> (add_mset h {#}) [] arr\<close>
+  shows \<open>encoded_hp_prop_list \<V> ((if remove_key a h = None then {#} else {#the (remove_key a h)#}) +
         (if find_key a h = None then {#} else {#the (find_key a h)#})) []
         arr'\<close>
 proof -
-  obtain prevs nxts childs parents scores \<V> where
+  obtain prevs nxts childs parents scores where
     arr: \<open>arr = ((prevs, nxts, childs, parents, scores))\<close> and
     dist: \<open>distinct_mset (mset_nodes h)\<close> and
-    \<V>: \<open>set_mset (sum_list (map mset_nodes xs)) \<subseteq> \<V>\<close>
+    \<V>: \<open>set_mset (mset_nodes h) \<subseteq> set_mset \<V>\<close>
     by (cases arr) (use assms in \<open>auto simp: ac_simps encoded_hp_prop_list2_conc_def encoded_hp_prop_list_def
         encoded_hp_prop_def\<close>)
   have find_key_in_nodes: \<open>find_key a h \<noteq> None \<Longrightarrow> node (the (find_key a h)) \<in># mset_nodes h\<close>
@@ -1959,6 +1983,15 @@ proof -
       using dist
       apply (auto simp: find_remove_mset_nodes_full)
       apply (metis distinct_mset_mono' mset_nodes_find_key_subset option.distinct(2) option.sel)
+      done
+  next
+    show \<open>set_mset (\<Sum>\<^sub># (mset_nodes `#
+     ((if remove_key a h = None then {#} else {#the (remove_key a h)#}) +
+      (if find_key a h = None then {#} else {#the (find_key a h)#})) +
+     mset_nodes `# mset []))
+      \<subseteq> set_mset \<V>\<close>
+      using \<V> apply (auto dest: in_find_key_in_nodes1)
+      apply (metis Set.basic_monos(7) in_remove_key_in_nodes option.distinct(2) option.sel)
       done
   next
     fix m' and x'
@@ -2745,7 +2778,7 @@ proof -
   obtain prevs nxts childs parents scores \<V> k where
     arr: \<open>arr = (\<V>, (prevs, nxts, childs, parents, scores), k)\<close> and
     dist: \<open>distinct_mset (mset_nodes (the h))\<close> and
-    k: \<open>k = Some (node (the h))\<close>\<open>the k \<in> \<V>\<close> and
+    k: \<open>k = Some (node (the h))\<close>\<open>the k \<in># \<V>\<close> and
     \<V>: \<open>set_mset ((mset_nodes (the h))) \<subseteq> \<V>\<close>
     by (cases arr; cases \<open>the h\<close>) (use assms in \<open>auto simp: ac_simps encoded_hp_prop_list2_conc_def encoded_hp_prop_list_def
       encoded_hp_prop_list_conc_def encoded_hp_prop_def\<close>)
@@ -2771,10 +2804,10 @@ proof -
    using enc 
    unfolding arr encoded_hp_prop_list_conc_def
    by (auto simp: encoded_hp_prop_def)
-  have KK': \<open>a\<in>#mset_nodes (the h) \<Longrightarrow> nxts a \<noteq> None \<Longrightarrow> the (nxts a) \<in> \<V>\<close>
-    \<open>a\<in>#mset_nodes (the h) \<Longrightarrow> prevs a \<noteq> None \<Longrightarrow> the (prevs a) \<in> \<V>\<close>
-    \<open>a\<in>#mset_nodes (the h) \<Longrightarrow> parents a \<noteq> None \<Longrightarrow> the (parents a) \<in> \<V>\<close>
-    \<open>a\<in>#mset_nodes (the h) \<Longrightarrow> childs a \<noteq> None \<Longrightarrow> the (childs a) \<in> \<V>\<close>
+  have KK': \<open>a\<in>#mset_nodes (the h) \<Longrightarrow> nxts a \<noteq> None \<Longrightarrow> the (nxts a) \<in># \<V>\<close>
+    \<open>a\<in>#mset_nodes (the h) \<Longrightarrow> prevs a \<noteq> None \<Longrightarrow> the (prevs a) \<in># \<V>\<close>
+    \<open>a\<in>#mset_nodes (the h) \<Longrightarrow> parents a \<noteq> None \<Longrightarrow> the (parents a) \<in># \<V>\<close>
+    \<open>a\<in>#mset_nodes (the h) \<Longrightarrow> childs a \<noteq> None \<Longrightarrow> the (childs a) \<in># \<V>\<close>
    using enc \<V> KK hp_next_in_nodes2[of a \<open>the h\<close> \<open>the (hp_next a (the h))\<close>] dist
      hp_parent_None_notin[of a \<open>the h\<close>]
      hp_prev_in_nodes[of a \<open>the h\<close>]
